Conditional Constant Propagation semantic proof

theories/Branch.v
@@ -8,19 +8,61 @@ Import Map MapF MapF.P MapF.P.F.
 Import IdOT MapCFG.
 
 Definition branches_aux (G: map_cfg) id b acc : list (blk*bid*bid*map_cfg) := match b.(blk_term) with
-    | TERM_Br _ l r => (b, l, r, (remove id G))::acc
-    | _ => acc
+  | TERM_Br _ l r => (b, l, r, (remove id G))::acc
+  | _ => acc
 end.
 
 Definition branches (G: map_cfg): list (blk*bid*bid*map_cfg) := fold (branches_aux G) G [].
 
-Record branch_sem (G G': map_cfg) (B:blk) l r: Prop := {
-    EQ: G' = (remove_id B G);
-    BR: exists e, B.(blk_term) = TERM_Br e l r
+Record branch_aux_sem (G0 G G': map_cfg) (B: blk) l r := {
+  EQ: G' = (remove_id B G0);
+  BR: exists e, B.(blk_term) = TERM_Br e l r;
+  MT: MapsTo_id B G
 }.
 
-Lemma branches_correct:
-    forall G G' b l r, wf_map_cfg G ->
-    (b,l,r,G') ∈ (branches G) <-> branch_sem G G' b l r.
+Definition branch_sem G G' B l r := branch_aux_sem G G G' B l r.
+
+Lemma branches_aux_correct:
+  forall G0 G G' b l r, wf_map_cfg G ->
+  (b, l , r, G') ∈ (fold (branches_aux G0) G []) <-> branch_aux_sem G0 G G' b l r.
 Proof.
-Admitted.
+  intros G0 G. apply fold_rec_bis.
+  - intros * EQ REC * WF'. assert (WF: wf_map_cfg m) by now apply (wf_map_cfg_eq m'). split.
+    * intros IN.
+      apply REC in IN as [EQ' [e TERM] MT]; trivial. repeat split; trivial.
+      now exists e. eapply MapsTo_m. 4: apply MT. reflexivity. trivial. now symmetry.
+    * intros [EQ' [e TERM] MT]. apply REC; trivial. repeat split; trivial. now exists e.
+      eapply MapsTo_m. 4: apply MT. all: auto. reflexivity.
+  - intros * WF. split. intro H. destruct H.
+    intros [EQ' [e TERM] MT]. now apply empty_mapsto_iff in MT.
+  - intros idB B * MT NIN REC * WFa.
+    assert (H: B.(blk_id) = idB). { apply WFa. now apply add_1. }
+    assert (WF': wf_map_cfg m'). { eapply add_wf_map_cfg. apply NIN. apply WFa. }
+    subst. split. 
+    * unfold branches_aux. intros IN. remember B.(blk_term) as T. induction T.
+      3: destruct IN as [EQ|IN].
+      3: {
+        apply pair_equal_spec in EQ as [EQ EQG].
+        apply pair_equal_spec in EQ as [EQ EQ1].
+        apply pair_equal_spec in EQ as [EQ EQ2]. subst.
+        repeat split; trivial. exists v. now rewrite HeqT.
+        now apply add_1. 
+      }
+      all: apply REC in IN as [EQ' [e TERM] MT']; trivial.
+      all: repeat split; trivial; [now exists e|].
+      all: apply add_2; [|apply MT'].
+      all: intros EQ; apply NIN; exists b.
+      all: apply eq_eq in EQ; rewrite EQ; apply MT'.
+    * intros [EQ' [e TERM] MT']. apply add_mapsto_iff in MT' as [[EQid EQb]|[NEQ MT']].
+      + subst b. unfold branches_aux. rewrite TERM. subst. now left.
+      + unfold branches_aux. remember B.(blk_term) as T. induction T.
+        3: right.
+        all: apply REC; trivial. all: split; trivial; now exists e.
+Qed.
+
+Lemma branches_correct:
+  forall G G' b l r, wf_map_cfg G ->
+  (b,l,r,G') ∈ (branches G) <-> branch_sem G G' b l r.
+Proof.
+  intros. now apply branches_aux_correct.
+Qed.
