theories/CCstP.v
@@ -10,10 +10,10 @@ Import IdOT MapCFG Head Focus Patterns.
 Notation exp := (texp dtyp).
 
 Inductive Analysis_1 : Type :=
-    | Top
-    | Bottom
-    | Zero
-    | One
+  | Top
+  | Bottom
+  | Zero
+  | One
 .
 
 Notation T := Top.
@@ -22,8 +22,32 @@ Notation "⊥" := Bottom.
 Definition analysis {S} := S -> Analysis_1.
 
 Definition fixed_branch (f:analysis) (b: blk) := match b.(blk_term) with
-    | TERM_Br e _ _ => match f e with | T | ⊥ => false | _ => true end
-    | _ => false
+  | TERM_Br e _ _ => match f e with | T | ⊥ => false | _ => true end
+  | _ => false
 end.
 
-Definition CCstP {S} (P:Pattern S) f := (Branch P) when (fun '(B,_,_,_) => fixed_branch f B).
+Definition CCstP {S} f (P:Pattern S) := (Branch P) when (fun '(B,_,_,_) => fixed_branch f B).
+
+Record CCstP_sem f (B: blk) G G' := {
+  WF: wf_map_cfg G';
+  EQ: G' = remove_id B G;
+  AN: exists e l r, B.(blk_term) = TERM_Br e l r /\ (f e = Zero \/ f e = One)
+}.
+
+Lemma Pattern_CCstP_correct {S}: forall f G B P (s:S), wf_map_cfg G ->
+    (exists l r, (B, l, r, s) ∈ (MatchAll (CCstP f P) G)) <->
+    exists G', s ∈ (MatchAll P G') /\ CCstP_sem f B G G'.
+Proof.
+  unfold CCstP. intros * WF. split.
+  - intros [l [r H]].
+    apply Pattern_When_correct in H as [H AN]. unfold fixed_branch in AN.
+    apply Pattern_Branch_correct in H as [G' [[EQ [e BR]] H]]; trivial.
+    exists G'. split; trivial.
+    rewrite BR in AN. repeat split; trivial. 2: exists e, l, r; split; trivial.
+    * rewrite EQ. now apply remove_wf_map_cfg.
+    * remember (f e) as a. induction a; try discriminate; auto.
+  - intros [G' [H [WF' EQ [e [l [r [EQT AN]]]]]]]. exists l, r.
+    apply Pattern_When_correct. split; trivial.
+    apply Pattern_Branch_correct; trivial. exists G'. repeat split; trivial.
+    now exists e. unfold fixed_branch. rewrite EQT. destruct AN as [AN|AN]; now rewrite AN.
+Qed.
